HASH-TABLE-EXPORT lemmas

books/projects/atomic-stobjs/lemmas/hash-table$a.lisp
@@ -35,6 +35,7 @@
 (local
   (include-book "std/omaps/top" :dir :system))
 
+(include-book "../utilities/with-books")
 (local
   (include-book "total-order"))
 (local
@@ -2265,3 +2266,767 @@
       :use ((:instance equal/unique
                        (%hash-table (cdr %hash-table))
                        (hash-table (cdr hash-table))))))))
+
+
+(local
+  (in-theory
+    (disable keysp
+             keys-fix
+             recognizer/unique
+             recognizer/copyable
+             creator/unique
+             (:e creator/unique)
+             creator/copyable
+             (:e creator/copyable)
+             fixer/unique
+             fixer/copyable
+             accessor/unique
+             accessor/copyable
+             updater/unique
+             updater/copyable
+             boundp/unique
+             boundp/copyable
+             getp/unique
+             getp/copyable
+             remover/unique
+             remover/copyable
+             count/unique
+             count/copyable
+             clear/unique
+             clear/copyable
+             init/unique
+             init/copyable
+             keys
+             keys-set
+             accessor/unique{definition}
+             updater/unique{definition}
+             boundp/unique{definition}
+             remover/unique{definition}
+             count/unique{definition}
+             recognizer/unique{induction}-fn
+             accessor/unique{induction}-fn
+             equal/unique
+             equal/copyable)))
+
+
+;;;; Value Export
+(encapsulate (((name) => *)
+              ((val-export-p *) => *)
+              ((val-export *) => *)
+              ((val-import * *) => *))
+  (local
+    (defun name ()
+      (declare (xargs :guard t))
+      nil))
+
+  (defthm name-constraint
+    (symbolp (name))
+    :rule-classes :type-prescription)
+
+  (local
+    (defun val-export-p (export)
+      (declare (xargs :guard t))
+      (val-recognizer export)))
+
+  (defthm val-export-p-constraint
+    (booleanp (val-export-p export))
+    :rule-classes :type-prescription)
+
+  (local
+    (defun val-export (val)
+      (declare (xargs :guard (val-recognizer val)))
+      (val-fixer val)))
+
+  (defthm val-export-p-of-val-export
+    (val-export-p (val-export val)))
+
+  (local
+    (defun val-import (export val)
+      (declare (xargs :guard (and (val-export-p export)
+                                  (val-recognizer val)))
+               (ignore val))
+      (val-fixer export)))
+
+  (defthm val-recognizer-of-val-import
+    (val-recognizer (val-import export val)))
+
+  (defthm val-import-when-not-val-export-p
+    (implies (not (val-export-p export))
+             (equal (val-import export val)
+                    (default-val))))
+
+  (defthmd val-import-ignores-val
+    (equal (val-import export val)
+           (val-import export (default-val))))
+
+  (defthm val-export-of-val-import
+    (implies (val-export-p export)
+             (equal (val-export (val-import export val))
+                    export)))
+
+  (defthm val-import-of-val-export
+    (equal (val-import (val-export %val) val)
+           (val-fixer %val))))
+
+
+;;;; `EXPORTP-REC'
+(defun exportp-rec (alist)
+  (declare (xargs :guard t))
+  (if (atom alist)
+      (null alist)
+      (and (consp (car alist))
+           (key-recognizer (caar alist))
+           (val-export-p (cdar alist))
+           (exportp-rec (cdr alist)))))
+
+(defthm exportp-rec{type-prescription}
+  (booleanp (exportp-rec alist))
+  :rule-classes :type-prescription)
+
+(defthm exportp-rec{compound-recognizer}
+  (implies (exportp-rec alist)
+           (true-listp alist))
+  :rule-classes :compound-recognizer)
+
+(defthm keysp-of-strip-cars-when-exportp-rec
+  (implies (exportp-rec alist)
+           (equal (keysp (strip-cars alist))
+                  (set::setp (strip-cars alist))))
+  :hints
+  (("Goal"
+    :in-theory (e/d (keysp
+                     set::head
+                     set::tail
+                     set::emptyp
+                     set::setp)
+                    (keysp{definition})))))
+
+(defthm key-recognizer-of-nth-when-exportp-rec
+  (implies (and (exportp-rec alist)
+                (natp n)
+                (< n (len alist)))
+           (key-recognizer (car (nth n alist)))))
+
+(defthm val-export-p-of-nth-when-exportp-rec
+  (implies (and (exportp-rec alist)
+                (natp n)
+                (< n (len alist)))
+           (val-export-p (cdr (nth n alist)))))
+
+(defthm alistp-when-exportp-rec
+  (implies (exportp-rec alist)
+           (alistp alist)))
+
+(defthm exportp-rec-of-cdr
+  (implies (and (exportp-rec alist)
+                (consp alist))
+           (exportp-rec (cdr alist))))
+
+(defthm val-export-p-of-assoc-when-exportp-rec
+  (implies (and (exportp-rec alist)
+                (assoc key alist))
+           (val-export-p (cdr (assoc key alist)))))
+
+
+;;;; `EXPORTP'
+(defun exportp (export)
+  (declare (xargs :guard t))
+  (and (consp export)
+       (equal (car export) (name))
+       (exportp-rec (cdr export))
+       (set::setp (strip-cars (cdr export)))))
+
+(defthm exportp{type-prescription}
+  (booleanp (exportp export))
+  :rule-classes :type-prescription)
+
+(defthm exportp{compound-recognizer}
+  (implies (exportp export)
+           (and (consp export)
+                (true-listp export)))
+  :rule-classes :compound-recognizer)
+
+(defthm car-when-exportp
+  (implies (exportp export)
+           (equal (car export)
+                  (name))))
+
+(defthm cdr-when-exportp
+  (implies (exportp export)
+           (and (exportp-rec (cdr export))
+                (keysp (strip-cars (cdr export))))))
+
+(defthm keysp-of-strip-cars-when-exportp
+  (implies (exportp alist)
+           (equal (keysp (strip-cars (cdr alist)))
+                  (set::setp (strip-cars (cdr alist)))))
+  :hints
+  (("Goal"
+    :do-not-induct t)))
+
+(defthm key-recognizer-of-nth-when-exportp
+  (implies (and (exportp alist)
+                (posp n)
+                (< n (len alist)))
+           (key-recognizer (car (nth n alist)))))
+
+(defthm val-export-p-of-nth-when-exportp
+  (implies (and (exportp alist)
+                (posp n)
+                (< n (len alist)))
+           (val-export-p (cdr (nth n alist)))))
+
+
+;;;; `EXPORT-ACC'
+(defun export-acc (set acc hash-table)
+  (declare (xargs :guard (and (keysp set)
+                              (exportp-rec acc)
+                              (recognizer/copyable hash-table))))
+  (if (set::emptyp set)
+      (revappend acc ())
+      (let* ((key (key-fixer (set::head set)))
+             (val (accessor/copyable key hash-table))
+             (export (val-export val)))
+        (export-acc (set::tail set) (acons key export acc) hash-table))))
+
+(defthm export-acc{type-prescription}
+  (implies (true-listp acc)
+           (true-listp (export-acc set acc hash-table)))
+  :rule-classes :type-prescription)
+
+(defthm export-acc-of-append
+  (equal (export-acc set (append %acc acc) hash-table)
+         (revappend acc (export-acc set %acc hash-table))))
+
+(defthm export-acc-factor
+  (implies (syntaxp (not (and (quotep acc)
+                              (equal (cadr acc) 'nil))))
+           (equal (export-acc set acc hash-table)
+                  (revappend acc (export-acc set () hash-table))))
+  :hints
+  (("Goal"
+    :in-theory (disable export-acc-of-append)
+    :use ((:instance export-acc-of-append
+                     (%acc ()))))))
+
+(defthm exportp-rec-of-export-acc
+  (implies (true-listp acc)
+           (equal (exportp-rec (export-acc set acc hash-table))
+                  (exportp-rec acc))))
+
+(defthm len-of-export-acc
+  (equal (len (export-acc set acc hash-table))
+         (+ (set::cardinality set) (len acc)))
+  :hints
+  (("Goal"
+    :in-theory (enable set::cardinality))))
+
+(with-books (("std/lists/append" :dir :system))
+  (defthm car-of-export-acc
+    (equal (car (export-acc set acc hash-table))
+           (cond
+             ((consp acc)
+              (nth (1- (len acc)) acc))
+             ((not (set::emptyp set))
+              (let ((key (key-fixer (set::head set))))
+                (cons key (val-export (accessor/copyable key hash-table)))))))
+    :hints
+    (("Goal"
+      :induct (len acc)
+      :in-theory (enable set::emptyp
+                         set::head
+                         set::tail)))))
+
+(defthm cdr-of-export-acc-when-atom
+  (implies (atom acc)
+           (equal (cdr (export-acc set acc hash-table))
+                  (and (not (set::emptyp set))
+                       (export-acc (set::tail set) () hash-table))))
+  :hints
+  (("Goal"
+    :do-not-induct t)
+   ("Subgoal 1"
+    :expand (EXPORT-ACC SET NIL HASH-TABLE))))
+
+(defthm consp-of-export-acc
+  (equal (consp (export-acc set acc hash-table))
+         (or (not (set::emptyp set))
+             (consp acc))))
+
+(with-books (("std/lists/append" :dir :system)
+             ("std/lists/nth" :dir :system))
+  (local
+    (defthm nth-of-export-acc-lemma-0
+      (implies (atom acc)
+               (equal (nth n (export-acc set acc hash-table))
+                      (and (< (nfix n) (set::cardinality set))
+                           (cons (key-fixer (nth n set))
+                                 (val-export (accessor/copyable (nth n set) hash-table))))))
+      :hints
+      (("Goal"
+        :in-theory (enable set::head
+                           set::tail
+                           set::emptyp
+                           set::cardinality)))))
+
+  (defthm nth-of-export-acc
+    (equal (nth n (export-acc set acc hash-table))
+           (cond
+             ((< (nfix n) (len acc))
+              (nth (- (len acc) (1+ (nfix n))) acc))
+             ((< (nfix n) (+ (set::cardinality set) (len acc)))
+              (let ((key (key-fixer (nth (- (nfix n) (len acc)) set))))
+                (cons key (val-export (accessor/copyable key hash-table)))))))
+    :hints
+    (("Goal"
+      :do-not-induct t))))
+
+(with-books (("std/alists/strip-cars" :dir :system))
+  (local
+    (defthm strip-cars-of-export-acc-when-atom
+      (implies (and (keysp set)
+                    (atom acc))
+               (equal (strip-cars (export-acc set acc hash-table))
+                      set))
+      :hints
+      (("Goal"
+        :in-theory (enable set::head
+                           set::tail
+                           set::setp
+                           set::emptyp
+                           keysp{definition})))))
+
+  (defthm strip-cars-of-export-acc
+    (implies (and (keysp set)
+                  (alistp acc))
+             (equal (strip-cars (export-acc set acc hash-table))
+                    (revappend (strip-cars acc) set)))
+    :hints
+    (("Goal"
+      :induct (strip-cars acc)))))
+
+
+;;;; `EXPORT'
+(defun export (hash-table)
+  (declare (xargs :guard (recognizer/copyable hash-table)))
+  (cons (name)
+        (export-acc (keys hash-table) () hash-table)))
+
+(defthm export{type-prescription}
+  (and (consp (export hash-table))
+       (true-listp (export hash-table)))
+  :rule-classes :type-prescription)
+
+(defthm exportp-of-export
+  (exportp (export hash-table)))
+
+(defthm len-of-export
+  (equal (len (export hash-table))
+         (1+ (set::cardinality (keys hash-table)))))
+
+(defthm nth-of-export
+  (equal (nth n (export hash-table))
+         (cond
+           ((zp n)
+            (name))
+           ((<= n (set::cardinality (keys hash-table)))
+            (let ((key (key-fixer (nth (1- n) (keys hash-table)))))
+              (cons key (val-export (accessor/copyable key hash-table)))))))
+  :hints
+  (("Goal"
+    :do-not-induct t
+    :expand (:free (n a d) (nth n (cons a d))))))
+
+(defthm strip-cars-of-export
+  (equal (strip-cars (cdr (export hash-table)))
+         (keys hash-table)))
+
+
+;;;; `IMPORT-REC'
+(defun import-rec (alist hash-table)
+  (declare (xargs :guard (and (exportp-rec alist)
+                              (recognizer/copyable hash-table))))
+  (if (atom alist)
+      (fixer/copyable hash-table)
+      (let* ((key (key-fixer (caar alist)))
+             (val (val-import (cdar alist) (default-val)))
+             (hash-table (updater/copyable key val hash-table)))
+        (import-rec (cdr alist) hash-table))))
+
+(defthm import-rec{type-prescription}
+  (and (consp (import-rec alist hash-table))
+       (true-listp (import-rec alist hash-table)))
+  :rule-classes :type-prescription)
+
+(defthm recognizer/copyable-of-import-rec
+  (recognizer/copyable (import-rec alist hash-table)))
+
+(defthm keys-of-import-rec
+  (equal (keys (import-rec alist hash-table))
+         (keys hash-table)))
+
+(defthm import-rec-of-updater/copyable
+  (implies (exportp-rec alist)
+           (equal (import-rec alist (updater/copyable key val hash-table))
+                  (if (assoc (key-fixer key) alist)
+                      (import-rec alist hash-table)
+                      (updater/copyable key val (import-rec alist hash-table))))))
+
+(defthm boundp/copyable-of-import-rec
+  (implies (exportp-rec alist)
+           (equal (boundp/copyable key (import-rec alist hash-table))
+                  (and (or (boundp/copyable key hash-table)
+                           (assoc (key-fixer key) alist))
+                       t)))
+  :hints
+  (("Goal"
+    :induct (exportp-rec alist))))
+
+(local
+  (encapsulate ()
+    (local
+      (defthm assoc-when-minimal-lemma-0
+        (implies (omap::mapp map)
+                 (equal (omap::assoc key map)
+                        (assoc key map)))
+        :hints
+        (("Goal"
+          :in-theory (enable omap::assoc
+                             omap::head
+                             omap::emptyp
+                             omap::mapp
+                             omap::tail)))))
+
+    (local
+      (in-theory
+        (enable omap::mapp-as-alistp)))
+
+    (defthmd assoc-when-minimal
+      (implies (and (alistp alist)
+                    (set::setp (strip-cars alist))
+                    (assoc key alist))
+               (not (<< key (caar alist))))
+      :hints
+      (("Subgoal *1/3"
+        :in-theory (e/d (omap::head
+                         mv-nth)
+                        (omap::head-key-minimal))
+        :use ((:instance omap::head-key-minimal
+                         (key key)
+                         (map alist))))))
+    (local
+      (defthm emptyp-when-setp
+        (implies (set::setp set)
+                 (equal (set::emptyp set)
+                        (null set)))
+        :hints
+        (("Goal"
+          :in-theory (enable set::setp
+                             set::emptyp)))))
+
+    (local
+      (in-theory
+        (enable assoc-when-minimal)))
+
+    (local
+      (defthm head-of-strip-cars
+        (implies (set::setp (strip-cars alist))
+                 (equal (set::head (strip-cars alist))
+                        (caar alist)))
+        :hints
+        (("Goal"
+          :in-theory (enable set::head)))))
+
+    (defthmd <<-when-setp-strip-cars
+      (implies (and (alistp alist)
+                    (consp alist)
+                    (consp (cdr alist))
+                    (not (<< (car (car alist)) (car (car (cdr alist))))))
+               (not (set::setp (strip-cars alist)))))
+
+    (local
+      (in-theory
+        (enable <<-when-setp-strip-cars)))
+
+    (local
+      (defthm car-of-strip-cars
+        (equal (car (strip-cars alist))
+               (caar alist))))
+
+    (defthmd assoc-when-setp-strip-cars
+      (implies (and (alistp alist)
+                    (consp alist)
+                    (assoc (car (car alist)) (cdr alist)))
+               (not (set::setp (strip-cars alist))))
+      :hints
+      (("Goal"
+        :do-not-induct t
+        :cases ((consp (cdr alist))))))
+
+    (local
+      (in-theory
+        (enable assoc-when-setp-strip-cars)))
+
+    (defthmd accessor/copyable-of-import-rec-lemma-0
+      (implies (and (exportp-rec alist)
+                    (set::setp (strip-cars alist))
+                    (key-recognizer key)
+                    (assoc key alist))
+               (equal (accessor/copyable key (import-rec alist hash-table))
+                      (val-import (cdr (assoc key alist))
+                                  (default-val))))
+      :hints
+      (("Goal"
+        :expand ((import-rec alist hash-table)))))))
+
+(defthm accessor/copyable-of-import-rec
+  (implies (and (exportp-rec alist)
+                (set::setp (strip-cars alist)))
+           (equal (accessor/copyable key (import-rec alist hash-table))
+                  (let ((pair (assoc (key-fixer key) alist)))
+                    (if pair
+                        (val-import (cdr pair) (default-val))
+                        (accessor/copyable key hash-table)))))
+  :hints
+  (("Goal"
+    :cases ((key-recognizer key)))
+   ("Subgoal 2.2"
+    :use ((:instance accessor/copyable-of-import-rec-lemma-0
+                     (key (default-key)))))
+   ("Subgoal 2.1"
+    :induct (import-rec alist hash-table))
+   ("Subgoal 1.2"
+    :use ((:instance accessor/copyable-of-import-rec-lemma-0)))
+   ("Subgoal 1.1"
+    :induct (import-rec alist hash-table))))
+
+(defthmd count/copyable-of-import-rec
+  (implies (and (exportp-rec alist)
+                (set::setp (strip-cars alist)))
+           (equal (count/copyable (import-rec alist hash-table))
+                  (cond
+                    ((atom alist)
+                     (count/copyable hash-table))
+                    ((boundp/copyable (caar alist) hash-table)
+                     (count/copyable (import-rec (cdr alist) hash-table)))
+                    (t
+                     (1+ (count/copyable (import-rec (cdr alist) hash-table)))))))
+  :hints
+  (("Goal"
+    :do-not-induct t
+    :in-theory (disable strip-cars))
+   ("Subgoal 1"
+    :use ((:instance assoc-when-setp-strip-cars))
+    :expand (import-rec alist hash-table))))
+
+
+;;;; `IMPORT'
+(defun import (export hash-table)
+  (declare (xargs :guard (and (exportp export)
+                              (recognizer/copyable hash-table))))
+  (if (exportp export)
+      (let* ((alist (cdr export))
+             (hash-table (clear/copyable hash-table))
+             (hash-table (import-rec alist hash-table))
+             (hash-table (keys-set (strip-cars alist) hash-table)))
+        hash-table)
+      (creator/copyable)))
+
+(defthm import{type-prescription}
+  (and (consp (import export hash-table))
+       (true-listp (import export hash-table)))
+  :rule-classes :type-prescription)
+
+(defthm recognizer/copyable-of-import
+  (recognizer/copyable (import export hash-table)))
+
+(defthm import-when-not-exportp
+  (implies (not (exportp export))
+           (equal (import export hash-table)
+                  (creator/copyable))))
+
+(defthmd import-ignores-hash-table
+  (equal (import export hash-table)
+         (import export (creator/copyable))))
+
+(defthm keys-of-import
+  (equal (keys (import export hash-table))
+         (and (exportp export)
+              (strip-cars (cdr export)))))
+
+(defthm boundp/copyable-of-import
+  (equal (boundp/copyable key (import export hash-table))
+         (and (assoc (key-fixer key) (cdr export))
+              (exportp export))))
+
+(defthm accessor/copyable-of-import
+  (equal (accessor/copyable key (import export hash-table))
+         (if (and (exportp export)
+                  (assoc (key-fixer key) (cdr export)))
+             (val-import (cdr (assoc (key-fixer key) (cdr export))) (default-val))
+             (default-val))))
+
+(local
+  (defthm setp-of-strip-cars-of-cdr
+    (implies (and (set::setp (strip-cars alist))
+                  (alistp alist)
+                  (consp alist))
+             (set::setp (strip-cars (cdr alist))))))
+
+(encapsulate ()
+  (local
+    (defthm count/copyable-of-import-lemma-0
+      (implies (and (exportp-rec alist)
+                    (set::setp (strip-cars alist)))
+               (equal (count/copyable (import-rec alist (creator/copyable)))
+                      (len alist)))
+      :hints
+      (("Goal"
+        :induct (len alist)
+        :expand (import-rec alist (creator/copyable)))
+       ("Subgoal *1/1.4"
+        :use ((:instance assoc-when-setp-strip-cars)))
+       ("Subgoal *1/1.2"
+        :use ((:instance assoc-when-setp-strip-cars))))))
+
+  (local
+    (defthmd count/copyable-of-import-lemma-1
+      (equal (count/copyable (import (cons (name) alist) hash-table))
+             (if (and (exportp-rec alist)
+                      (set::setp (strip-cars alist)))
+                 (len alist)
+                 0))
+      :hints
+      (("Goal"
+        :in-theory (disable exportp-rec
+                            strip-cars
+                            key-fixer-constraint)))))
+
+  (defthm count/copyable-of-import
+    (equal (count/copyable (import export hash-table))
+           (if (exportp export)
+               (1- (len export))
+               0))
+    :hints
+    (("Goal"
+      :do-not-induct t
+      :use ((:instance count/copyable-of-import-lemma-1
+                       (alist (cdr export))))))))
+
+
+;;;; `EXPORT' and `IMPORT' Composition Theorems
+(with-books (("std/lists/nth" :dir :system)
+             ("std/alists/strip-cars" :dir :system))
+  (local
+    (defthm cardinality-is-len
+      (implies (set::setp set)
+               (equal (set::cardinality set)
+                      (len set)))
+      :hints
+      (("Goal"
+        :in-theory (enable set::cardinality
+                           set::tail
+                           set::emptyp)))))
+
+  (local
+    (defthm nth-of-strip-cars
+      (equal (nth n (strip-cars alist))
+             (car (nth n alist)))))
+
+  (local
+    (defthmd equal-cons
+      (implies (consp c)
+               (equal (equal (cons a d)
+                             c)
+                      (and (equal a (car c))
+                           (equal d (cdr c)))))))
+
+  (local
+    (defthm consp-of-nth-when-alistp
+      (implies (and (alistp alist)
+                    (natp n)
+                    (< n (len alist)))
+               (consp (nth n alist)))))
+
+  (local
+    (defthm assoc-of-nth-when-alistp
+      (implies (and (alistp alist)
+                    (natp n)
+                    (< n (len alist)))
+               (assoc (car (nth n alist)) alist))))
+
+  (local
+    (defthm assoc-of-nth-when-exportp-rec
+      (implies (and (exportp-rec alist)
+                    (set::setp (strip-cars alist))
+                    (natp n)
+                    (< n (len alist)))
+               (equal (assoc-equal (car (nth n alist)) alist)
+                      (nth n alist)))
+      :hints
+      (("Goal"
+        :induct (nth n alist))
+       ("Subgoal *1/3"
+        :in-theory (disable consp-of-nth-when-alistp)
+        :use ((:instance assoc-when-setp-strip-cars)
+              (:instance consp-of-nth-when-alistp
+                         (n (+ -1 n))
+                         (alist (cdr alist))))))))
+
+  (defthm export-of-import
+    (implies (exportp export)
+             (equal (export (import export hash-table))
+                    export))
+    :hints
+    ((acl2::equal-by-nths-hint)
+     ("Goal"
+      :in-theory (disable exportp-rec
+                          export-acc
+                          import-rec)
+      :expand (:free (n a d) (nth n (cons a d))))
+     ("Subgoal 1.2"
+      :use ((:instance consp-of-nth-when-alistp
+                       (n (+ -1 acl2::n))
+                       (alist (cdr export))))))))
+
+(defthm import-of-export
+  ;; We assume that `%HASH-TABLE' is coupled.
+  (implies (and (equal (set::cardinality (keys %hash-table))
+                       (count/copyable %hash-table))
+                (iff (assoc-equal
+                      (keys-equal/copyable-witness (import (export %hash-table) hash-table)
+                                                   (fixer/copyable %hash-table))
+                      (cdr (export %hash-table)))
+                     (boundp/copyable
+                      (keys-equal/copyable-witness (import (export %hash-table) hash-table)
+                                                   (fixer/copyable %hash-table))
+                      %hash-table))
+                (iff (assoc-equal
+                      (vals-equal/copyable-witness (import (export %hash-table) hash-table)
+                                                   (fixer/copyable %hash-table))
+                      (cdr (export %hash-table)))
+                     (boundp/copyable
+                      (vals-equal/copyable-witness (import (export %hash-table) hash-table)
+                                                   (fixer/copyable %hash-table))
+                      %hash-table))
+                (equal
+                 (val-import
+                  (cdr
+                   (assoc-equal
+                    (vals-equal/copyable-witness (import (export %hash-table) hash-table)
+                                                 (fixer/copyable %hash-table))
+                    (cdr (export %hash-table))))
+                  (default-val))
+                 (accessor/copyable
+                  (vals-equal/copyable-witness (import (export %hash-table) hash-table)
+                                               (fixer/copyable %hash-table))
+                  %hash-table)))
+           (equal (import (export %hash-table) hash-table)
+                  (fixer/copyable %hash-table)))
+  :hints
+  (("Goal"
+    :in-theory (disable import
+                        export)
+    :use ((:instance equal/copyable
+                     (%hash-table (import (export %hash-table) hash-table))
+                     (hash-table (fixer/copyable %hash-table)))))))
